Refactor state updates to be explicit pure functions
These are much easier to prove than the mutable ref variant, which seems impossible because the
details of ST and IO are not exposed.  Make the state updates explicit for now.  The extractor to
elisp can handle turning those into mutable updates (or just letting the caller do it explicitly).

LgtmLean/LgtmLean/Interface.lean
@@ -5,23 +5,25 @@ import Std
 public import LgtmLean.Basic
 public import LgtmLean.CreateThreads
 
+public structure Result α where
+  value : α
+  updatedState : State
 
 /-- Delete all of the comments in the current review state.
 
 This is used to prepare to fetch an updated state from the server. -/
-public def resetCommentState : LgtmM Unit := do
-  let s₀ ← getState
+public def resetCommentState (s₀ : State) : Result Unit :=
   let manager₁ := s₀.fileManager.resetCommentState
-  setState { s₀ with
-    commentBeingEdited := none,
-    commentManager := CommentManager.empty,
-    fileManager := manager₁,
-    hCommentBeingEditedWellFormed := by simp,
-    hFileThreadsPublished := s₀.fileManager.hFileThreadsPublished_resetCommentState CommentManager.empty.comments }
+  let s₁ := { s₀ with
+              commentBeingEdited := none,
+              commentManager := CommentManager.empty,
+              fileManager := manager₁,
+              hCommentBeingEditedWellFormed := by simp,
+              hFileThreadsPublished := s₀.fileManager.hFileThreadsPublished_resetCommentState CommentManager.empty.comments }
+  Result.mk () s₁
 
 
-public def addRemoteComments (comments : List Comment) : LgtmM Unit := do
-  pure ()
+public def addRemoteComments (s₀ : State) (comments : List Comment) : Result Unit := sorry
 
 /-- The core worker called to update the state when the user marks a comment as done.
 
@@ -40,18 +42,17 @@ Note that we could add a proof obligation that the content is not empty, but thi
 context outside of the context of the Lean code, so that proof obligation cannot be fulfilled.
 
 -/
-public def completeCommentWithContent (newContent : String) : LgtmM (Except String Comment) := do
+public def completeCommentWithContent (s₀ : State) (newContent : String) : Result (Except String Comment) :=
   if newContent.isEmpty then
-    pure (Except.error "Comments cannot be empty")
+    Result.mk (Except.error "Comments cannot be empty") s₀
   else
-    let s₀ ← getState
     match hBeingEdited : s₀.commentBeingEdited with
-    | none => pure (Except.error "No active comment")
+    | none => Result.mk (Except.error "No active comment") s₀
     | some editedCommentRef =>
       let comment₀ := s₀.commentManager.get editedCommentRef
       let comment₁ := { comment₀ with content := newContent }
       match s₀.configuration.createComment comment₁ with
-      | none => pure (Except.error "Failed to create the comment on the server")
+      | none => Result.mk (Except.error "Failed to create the comment on the server") s₀
       | some serverId =>
         let comment₂ : Comment := { comment₁ with backendId := serverId }
         have hbackendId2 : comment₂.backendId = some serverId := rfl
@@ -135,15 +136,15 @@ public def completeCommentWithContent (newContent : String) : LgtmM (Except Stri
               hCommentsKeyedByRef := hCommentsKeyedByRef₁,
               hTopLevelThreadsAllTopLevel := hTopLevelThreadsAllTopLevel₁,
               hTopLevelThreadsPublished := hTopLevelThreadsPublished₁ }
-          setState { s₀ with
-            commentBeingEdited := none,
-            commentManager := commentManager₁,
-            hCommentBeingEditedWellFormed := by simp,
-            hFileThreadsPublished := hFileThreadsPublished₁ }
-          pure (Except.ok comment₂)
+          let s₁ := { s₀ with
+                      commentBeingEdited := none,
+                      commentManager := commentManager₁,
+                      hCommentBeingEditedWellFormed := by simp,
+                      hFileThreadsPublished := hFileThreadsPublished₁ }
+          Result.mk (Except.ok comment₂) s₁
         | .fileLocation loc =>
           match hfound : s₀.fileManager.state.toList.find? (λ (_, modifiedFileState) => modifiedFileState.fileRef == loc.fileRef) with
-          | none => pure (Except.error "Unexpected file")
+          | none => Result.mk (Except.error "Unexpected file") s₀
           | some (fileRef, modifiedFileState) =>
             have hFound := s₀.fileManager.contains_get_of_find? hfound
             have hOldContainsFileRef := hFound.1
@@ -236,13 +237,13 @@ public def completeCommentWithContent (newContent : String) : LgtmM (Except Stri
                 { s₀.fileManager with
                   state := newState,
                   hConsistentState := hConsistentState₁ }
-              setState { s₀ with
-                commentBeingEdited := none,
-                commentManager := commentManager₁,
-                fileManager := fileManager₁,
-                hCommentBeingEditedWellFormed := by simp,
-                hFileThreadsPublished := hFileThreadsPublished₂ }
-              pure (Except.ok comment₂)
+              let s₁ := { s₀ with
+                          commentBeingEdited := none,
+                          commentManager := commentManager₁,
+                          fileManager := fileManager₁,
+                          hCommentBeingEditedWellFormed := by simp,
+                          hFileThreadsPublished := hFileThreadsPublished₂ }
+              Result.mk (Except.ok comment₂) s₁
             | .current =>
               have hparentCurrent : ∀ parentId, comment₂.parent = some parentId →
                   parentId ∈ modifiedFileState.currentThreads.serverCommentIds := by
@@ -286,10 +287,18 @@ public def completeCommentWithContent (newContent : String) : LgtmM (Except Stri
                 { s₀.fileManager with
                   state := newState,
                   hConsistentState := hConsistentState₁ }
-              setState { s₀ with
-                commentBeingEdited := none,
-                commentManager := commentManager₁,
-                fileManager := fileManager₁,
-                hCommentBeingEditedWellFormed := by simp,
-                hFileThreadsPublished := hFileThreadsPublished₂ }
-              pure (Except.ok comment₂)
+              let s₁ := { s₀ with
+                          commentBeingEdited := none,
+                          commentManager := commentManager₁,
+                          fileManager := fileManager₁,
+                          hCommentBeingEditedWellFormed := by simp,
+                          hFileThreadsPublished := hFileThreadsPublished₂ }
+              Result.mk (Except.ok comment₂) s₁
+
+private theorem completeCommentWithContent.rejectsEmptyContent (s₀ : State) :
+  ∃ msg result, completeCommentWithContent s₀ "" = result ∧ result.value = Except.error msg :=
+    ⟨"Comments cannot be empty", _, rfl, rfl⟩
+
+private theorem completeCommentWithContent.preservesStateWithEmptyContent (s₀ : State) :
+  ∃ result, completeCommentWithContent s₀ "" = result ∧ result.updatedState = s₀ :=
+    ⟨_, rfl, rfl⟩
